\section{Two Dimensions}
Let 
\begin{equation}
\mbf{y} = A\mbf{x} + \mbf{n},
\end{equation}
where 
\begin{align}
x &\in \brak{\mbf{s}_0,\mbf{s}_1}, 
\mbf{s}_0 = 
\begin{pmatrix}
1 
\\
0
\end{pmatrix},
\mbf{s}_1 = 
\begin{pmatrix}
0 
\\
1
\end{pmatrix}
\\
\mbf{n} &= 
\begin{pmatrix}
n_1
\\
n_2
\end{pmatrix},
n_1,n_2 \sim \gauss{0}{1}.
\end{align}
%
\begin{enumerate}
%%
\item
\label{ch5_fsk}
Plot 
%
\begin{equation}
\mbf{y}|\mbf{s}_0 \text{ and } \mbf{y}|\mbf{s}_1
\end{equation}
%
on the same graph using a scatter plot.\\
\solution The scatter plot in \figref{fig:biv_scatter} is generated using the below code,
\begin{lstlisting}
chapter5/codes/biv_scatter.py
\end{lstlisting}
%
\begin{figure}[H]
\centering
\includegraphics[width=\columnwidth]{chapter5/figs/biv_scatter.pdf}
\caption{Scatter plot of $\mbf{y}|\mbf{s}_0$ and $\mbf{y}|\mbf{s}_1$ }
\label{fig:biv_scatter}
\end{figure}

%
\item
For the above problem, find a decision rule for detecting the symbols $\mbf{s}_0 $ and $\mbf{s}_1$.\\
\solution Let $\mbf{y} = \myvec{y_1&y_2}^T$. Then the decision rule is
\begin{equation}
	y_1 \dec{0}{1} y_2
	\label{eq:biv_fsk_decision}
\end{equation}
%$\vec{y}|\vec{s}_i$ is a random vector with each of its components normally distributed. The PDF of $\vec{y}|\vec{s}_i$ is given by,
\begin{equation}
	p_{\vec{y}|\vec{s}_i}\brak{\vec{y}} = \frac{1}{2\pi\sqrt{\mydet{\vec{\Sigma}}}} \exp\brak{-\frac{1}{2}\brak{\vec{y}-\vec{s}_i}^\top \vec{\Sigma}^{-1} \brak{\vec{y}-\vec{s}_i}}
\end{equation}
Where $\vec{\Sigma}$ is the covariance matrix. Substituting $\vec{\Sigma} = \sigma \vec{I}$,
\begin{align}
	p_{\vec{y}|\vec{s}_i}\brak{\vec{y}} &= \frac{1}{2 \pi \sigma} \exp\brak{-\frac{1}{2 \sigma}\brak{\vec{y}-\vec{s}_i}^\top \vec{I} \brak{\vec{y}-\vec{s}_i}}\\
	&= \frac{1}{2 \pi \sigma} \exp\brak{-\frac{1}{2 \sigma}\brak{\vec{y}-\vec{s}_i}^\top \brak{\vec{y}-\vec{s}_i}}
\end{align}
Assuming equiprobable symbols, use MAP rule to find optimum decision. Since there are only two possible symbols %
$\vec{s}_0$ and $\vec{s}_1$, the optimal decision criterion is found by equating $p_{\vec{y}|\vec{s}_0}$ and $p_{\vec{y}|\vec{s}_1}$.
\begin{align*}
	p_{\vec{y}|\vec{s}_0} &= p_{\vec{y}|\vec{s}_1}
\end{align*}
	
\begin{multline*}
	\implies \exp\brak{-\frac{1}{2 \sigma}\brak{\vec{y}-\vec{s}_0}^\top \brak{\vec{y}-\vec{s}_0}} = \\
	\exp\brak{-\frac{1}{2 \sigma}\brak{\vec{y}-\vec{s}_1}^\top \brak{\vec{y}-\vec{s}_1}}
\end{multline*}
	
\begin{align*}
	\implies \brak{\vec{y}-\vec{s}_0}^\top \brak{\vec{y}-\vec{s}_0} &= \brak{\vec{y}-\vec{s}_1}^\top \brak{\vec{y}-\vec{s}_1}\\
	\implies \vec{y}^\top\vec{y} - 2\vec{s}_0^\top \vec{y} + \vec{s}_0^T\vec{s}_0 &= \vec{y}^\top\vec{y} - 2\vec{s}_1^\top \vec{y} + \vec{s}_1^T\vec{s}_1\\
	\implies 2\brak{\vec{s}_1-\vec{s}_0}^\top \vec{y} &= \norm{\vec{s}_1}^2 - \norm{\vec{s}_0}^2\\
	\implies \brak{\vec{s}_1-\vec{s}_0}^\top \vec{y} &= 0\\
	\implies \myvec{-1\\1}^\top \vec{y} &= 0
\end{align*}
%
\item
Plot 
\begin{equation} 
P_e = \pr{\hat{\mbf{x}} = \mbf{s}_1|\mbf{x} = \mbf{s}_0}
\label{eq:prob_error_fsk}
\end{equation}
with respect to the SNR from 0 to 10 dB.\\
\solution The blue dots in \figref{fig:biv_pe_snr} are the $P_e$ versus SNR plot. It is generated using the below code,
\begin{lstlisting}
chapter5/codes/biv_pe_snr.py
\end{lstlisting}
%
\item
Obtain an expression for $P_e$. Verify this by comparing the theory and simulation plots on the same graph.\\
\solution Using the decision rule from \eqref{eq:biv_fsk_decision},
\begin{align}
	\nonumber
	P_e &= \pr{\hat{\mbf{x}} = \mbf{s}_1|\mbf{x} = \mbf{s}_0}\\\nonumber
	&= \pr{y_1 < y_2|\mbf{x} = \mbf{s}_0}\\\nonumber
	&= \pr{A+n_1 < n_2}\\
	\label{eq:prob_error_fsk_inter}
	&= \pr{n_1-n_2 < -A}
\end{align}
%\textbf{Theorem:} The sum of $N$ independant random variables $X_1,X_2,...,X_N$ with $X_i \sim \gauss{\mu_i}{\sigma_i}$ is itself normally distributed %
%with $\mu =\sum_{i=1}^n \mu_i$ and $\sigma^2 = \sum_{i=1}^n \sigma_i^2$.\\
Let $Z = n_1-n_2$ where $n_1, n_2 \sim \gauss{0}{\sigma^2}$. The PDF of X is given by,
\begin{align}
	\nonumber
	p_Z(z) &= p_{n_1}(n_1) \ast p_{-n_2}(n_2)\\\nonumber
	&= \frac{1}{2\pi\sigma^2}\int_{-\infty}^{\infty} e^{-\frac{t^2}{2\sigma^2}}e^{-\frac{(t-z)^2}{2\sigma^2}}  \,dt\\\nonumber
	&= \frac{1}{2\pi\sigma^2}\int_{-\infty}^{\infty} e^{-\frac{(z-t)^2+t^2}{2\sigma^2}}  \,dt\\\nonumber
	&= \frac{1}{2\pi\sigma^2}\int_{-\infty}^{\infty} e^{-\frac{(2t-z)^2+z^2}{2(\sqrt{2}\sigma)^2}}  \,dt\\\nonumber
	&= \frac{1}{2\pi\sigma^2}e^{-\frac{z^2}{2(\sqrt{2}\sigma)^2}}\int_{-\infty}^{\infty} e^{-\frac{(2t-z)^2}{2(\sqrt{2}\sigma)^2}}  \,dt\\\nonumber
	&= \frac{e^{-\frac{z^2}{2(\sqrt{2}\sigma)^2}}}{\sqrt{2\pi}\sqrt{2}\sigma} \frac{1}{\sqrt{2\pi}\sqrt{2}\sigma}\int_{-\infty}^{\infty} e^{-\frac{k^2}{2(\sqrt{2}\sigma)^2}}  \,dk\\
	\label{eq:std_gauss_diff_pdf_fsk}
	&= \frac{e^{-\frac{z^2}{2(\sqrt{2}\sigma)^2}}}{\sqrt{2\pi}\sqrt{2}\sigma}
\end{align}
From \eqref{eq:std_gauss_diff_pdf_fsk}, $Z \sim \gauss{0}{2\sigma^2}$. Substituting $\sigma=1$, $Z \sim \gauss{0}{2}$. %
\eqref{eq:prob_error_fsk_inter} can be further simplified as,
\begin{align*}
	P_e &= \pr{Z < -A}&\\
	&= \pr{Z > A}&\\
	&= \qfunc{\frac{A}{\sqrt{2}}}&\\
	&= \frac{1}{\sqrt{2\pi}}\int_{\frac{A}{\sqrt{2}}}^{\infty} \exp\left(-\frac{x^2}{2}\right)  \,dx 
\end{align*}
\figref{fig:biv_pe_snr} compares the theoretical and simulation plots.

\begin{figure}[H]
\centering
\includegraphics[width=\columnwidth]{chapter5/figs/biv_pe_vs_snr.pdf}
\caption{$P_e$ versus SNR plot for FSK}
\label{fig:biv_pe_snr}
\end{figure}
%
\end{enumerate}
